start formalizing 'red_inhale'
Progress:
* Inhaling predicate missing.
* Needs to decide if 'red_inhale' checks satisfiability or consistency.

viper-total-heaps/TotalSemantics.thy
@@ -4,6 +4,65 @@ theory TotalSemantics
 imports ViperCommon.ViperLang TotalSemanticsCore "HOL-Eisbach.Eisbach" "HOL-Eisbach.Eisbach_Tools"
 begin
 
+subsection \<open>General Auxiliary Definitions\<close>
+
+datatype 'a stmt_result_total = RMagic | RFailure | RNormal "'a full_total_state"
+
+fun map_stmt_result_total :: "('a full_total_state \<Rightarrow> 'b full_total_state) \<Rightarrow> 'a stmt_result_total \<Rightarrow> 'b stmt_result_total"
+  where
+    "map_stmt_result_total f (RNormal \<omega>) = (RNormal (f \<omega>))"
+  | "map_stmt_result_total f RMagic = RMagic"
+  | "map_stmt_result_total f RFailure = RFailure"
+
+inductive th_result_rel :: "bool \<Rightarrow> bool \<Rightarrow> ('a full_total_state) set \<Rightarrow> 'a stmt_result_total \<Rightarrow> bool"  where
+  THResultNormal: "\<lbrakk> \<omega> \<in> W \<rbrakk> \<Longrightarrow> th_result_rel True True W (RNormal \<omega>)"
+| THResultMagic: "th_result_rel True False W RMagic"
+| THResultFailure: "th_result_rel False b W RFailure"
+
+text \<open>\<^const>\<open>th_result_rel\<close> is an auxiliary relation that is useful to express a state in terms of
+conditions. \<^term>\<open>th_result_rel bSuccess bFeasible W res\<close> is used in the following way:
+
+  \<^item> \<^term>\<open>bSuccess\<close> expresses when \<^term>\<open>res\<close> is not a failing state
+  \<^item> If \<^term>\<open>bSuccess\<close> holds (i.e., \<^term>\<open>res\<close> not a failing state), then
+    \<^term>\<open>bFeasible\<close> expresses when res is a normal state.
+  \<^item> W expresses the set of possible normal states for \<^term>\<open>res\<close> if both \<^term>\<open>bSuccess\<close> and
+    \<^term>\<open>bFeasible\<close> hold.
+\<close>
+
+inductive_cases THResultNormal_case: "th_result_rel True True W (RNormal \<omega>)"
+thm THResultNormal_case
+
+lemma THResultNormal_alt: "\<lbrakk> \<omega> \<in> W; A; B\<rbrakk> \<Longrightarrow> th_result_rel A B W (RNormal \<omega>)"
+  by (cases A; cases B) (auto intro: THResultNormal)
+
+lemma th_result_rel_normal:
+  assumes "th_result_rel a b W (RNormal \<omega>)"
+  shows "a \<and> b \<and> \<omega> \<in> W"
+  using assms
+  by (cases) auto
+
+text \<open>\<^typ>\<open>'a stmt_result_total\<close> expresses the possible states for statements. \<close>
+
+
+lemma th_result_rel_failure:
+  assumes "th_result_rel False b W res"
+  shows "res = RFailure"
+  using assms
+  by (cases) auto
+
+lemma th_result_rel_failure_2:
+  assumes "th_result_rel a b W RFailure"
+  shows "\<not>a"
+  using assms
+  by (cases) auto
+
+lemma th_result_rel_magic:
+  assumes "th_result_rel True False W res"
+  shows "res = RMagic"
+  using assms
+  by (cases) auto
+
+
 definition vals_well_typed :: "('a \<Rightarrow> abs_type) \<Rightarrow> ('a val) list \<Rightarrow> vtyp list \<Rightarrow> bool"
   where "vals_well_typed A vs ts \<equiv> map (get_type A) vs = ts"
 
@@ -38,7 +97,7 @@ lemma exh_if_total_failure:
 
 definition exhale_perm_single :: "preal mask \<Rightarrow> heap_loc \<Rightarrow> preal option \<Rightarrow> (preal mask) set"
   where "exhale_perm_single m lh p_opt =
-      {m'| m' q. 
+      {m'| m' q.
                (p_opt = None \<longrightarrow> pgt q pnone) \<and>
                option_fold ((=) q) (q \<noteq> pnone \<and> pgt (m lh) q) p_opt \<and>
                m' = m(lh := (m lh) - q)
@@ -49,12 +108,12 @@ inductive red_exhale :: "'a total_context \<Rightarrow> ('a full_total_state \<R
   where
 
 \<comment>\<open>exhale acc(e.f, p)\<close>
-  ExhAcc: 
+  ExhAcc:
   "\<lbrakk>  mh = get_mh_total_full \<omega>;
-     ctxt, R, (Some \<omega>0) \<turnstile> \<langle>e_r; \<omega>\<rangle> [\<Down>]\<^sub>t Val (VRef r); 
-     ctxt, R, (Some \<omega>0) \<turnstile> \<langle>e_p; \<omega>\<rangle> [\<Down>]\<^sub>t Val (VPerm p);
+     ctxt, (Some \<omega>0) \<turnstile> \<langle>e_r; \<omega>\<rangle> [\<Down>]\<^sub>t Val (VRef r);
+     ctxt, (Some \<omega>0) \<turnstile> \<langle>e_p; \<omega>\<rangle> [\<Down>]\<^sub>t Val (VPerm p);
      a = the_address r \<rbrakk> \<Longrightarrow>
-     red_exhale ctxt R \<omega>0 (Atomic (Acc e_r f (PureExp e_p))) \<omega> 
+     red_exhale ctxt R \<omega>0 (Atomic (Acc e_r f (PureExp e_p))) \<omega>
                           ( exh_if_total (p \<ge> 0 \<and> (if r = Null then p = 0 else pgte (mh (a,f)) (Abs_preal p)))
                                          (if r = Null then \<omega> else update_mh_loc_total_full \<omega> (a,f) ((mh (a,f)) - (Abs_preal p)))
                           )"
@@ -62,27 +121,27 @@ inductive red_exhale :: "'a total_context \<Rightarrow> ('a full_total_state \<R
 \<comment>\<open>Exhaling wildcard removes some non-zero permission that is less than the current permission held.\<close>
 | ExhAccWildcard:
   "\<lbrakk> mh = get_mh_total_full \<omega>;
-     ctxt, R, (Some \<omega>0) \<turnstile> \<langle>e_r; \<omega>\<rangle> [\<Down>]\<^sub>t Val (VRef r);
+     ctxt, (Some \<omega>0) \<turnstile> \<langle>e_r; \<omega>\<rangle> [\<Down>]\<^sub>t Val (VRef r);
      a = the_address r;
-     \<comment>\<open>\<^term>\<open>q\<close> satisfies the right-hand side if \<^prop>\<open>mh (a,f) \<noteq> pnone\<close> (thm prat_exists_stricly_smaller_nonzero). 
+     \<comment>\<open>\<^term>\<open>q\<close> satisfies the right-hand side if \<^prop>\<open>mh (a,f) \<noteq> pnone\<close> (thm prat_exists_stricly_smaller_nonzero).
      If \<^prop>\<open>mh (a,f) \<noteq> pnone\<close> does not hold, then the exhale fails and the value of q is irrelevant. \<close>
-     q = (SOME p. p \<noteq> pnone \<and> pgt (mh (a,f)) p) 
+     q = (SOME p. p \<noteq> pnone \<and> pgt (mh (a,f)) p)
    \<rbrakk> \<Longrightarrow>
      red_exhale ctxt R \<omega>0 (Atomic (Acc e_r f Wildcard)) \<omega>
-                         (exh_if_total (mh (a,f) \<noteq> pnone \<and> r \<noteq> Null) 
+                         (exh_if_total (mh (a,f) \<noteq> pnone \<and> r \<noteq> Null)
                                        (update_mh_loc_total_full \<omega> (a,f) q))"
 \<comment>\<open>exhale acc(P(es), p)\<close>
 | ExhAccPred:
    "\<lbrakk> mp = get_mp_total_full \<omega>;
      red_pure_exps_total ctxt R (Some \<omega>0) e_args \<omega> (Some v_args);
-     ctxt, R, (Some \<omega>0) \<turnstile> \<langle>e_p; \<omega>\<rangle> [\<Down>]\<^sub>t Val (VPerm p) \<rbrakk> \<Longrightarrow>
+     ctxt, (Some \<omega>0) \<turnstile> \<langle>e_p; \<omega>\<rangle> [\<Down>]\<^sub>t Val (VPerm p) \<rbrakk> \<Longrightarrow>
      red_exhale ctxt R \<omega>0 (Atomic (AccPredicate pred_id e_args (PureExp e_p))) \<omega>
-            (exh_if_total (p \<ge> 0 \<and> pgte (mp(pred_id, v_args)) (Abs_preal p)) 
+            (exh_if_total (p \<ge> 0 \<and> pgte (mp(pred_id, v_args)) (Abs_preal p))
                           (update_mp_loc_total_full \<omega> (pred_id, v_args) (mp (pred_id, v_args) - (Abs_preal p))))"
 | ExhAccPredWildcard:
   "\<lbrakk> mp = get_mp_total_full \<omega>;
      red_pure_exps_total ctxt R (Some \<omega>0) e_args \<omega> (Some v_args);
-    \<comment>\<open>q satisfies the right-hand side if \<^prop>\<open>mp (pred_id, v_args) \<noteq> pnone\<close> (thm prat_exists_stricly_smaller_nonzero). 
+    \<comment>\<open>q satisfies the right-hand side if \<^prop>\<open>mp (pred_id, v_args) \<noteq> pnone\<close> (thm prat_exists_stricly_smaller_nonzero).
      If \<^prop>\<open>mp (pred_id, v_args) \<noteq> pnone\<close> does not hold, then the exhale fails and the value of q is irrelevant.\<close>
      q = (SOME p. p \<noteq> pnone \<and> pgt (mp (pred_id, v_args)) p)
    \<rbrakk> \<Longrightarrow>
@@ -91,51 +150,51 @@ inductive red_exhale :: "'a total_context \<Rightarrow> ('a full_total_state \<R
                                        (update_mp_loc_total_full \<omega> (pred_id, v_args) q))"
 
 | ExhPure:
-  "\<lbrakk> ctxt, R, (Some \<omega>0) \<turnstile> \<langle>e; \<omega>\<rangle> [\<Down>]\<^sub>t Val (VBool b) \<rbrakk> \<Longrightarrow>
+  "\<lbrakk> ctxt, (Some \<omega>0) \<turnstile> \<langle>e; \<omega>\<rangle> [\<Down>]\<^sub>t Val (VBool b) \<rbrakk> \<Longrightarrow>
      red_exhale ctxt R \<omega>0 (Atomic (Pure e)) \<omega> (exh_if_total b \<omega>)"
 
 \<comment>\<open>exhale A && B\<close>
-| ExhStarNormal: 
- "\<lbrakk> red_exhale ctxt R \<omega>0 A \<omega> (RNormal \<omega>'); 
+| ExhStarNormal:
+ "\<lbrakk> red_exhale ctxt R \<omega>0 A \<omega> (RNormal \<omega>');
     red_exhale ctxt R \<omega>0 B \<omega>' res\<rbrakk> \<Longrightarrow>
     red_exhale ctxt R \<omega>0 (A && B) \<omega> res"
-| ExhStarFailure: 
+| ExhStarFailure:
  "\<lbrakk> red_exhale ctxt R \<omega>0 A \<omega> RFailure \<rbrakk> \<Longrightarrow>
     red_exhale ctxt R \<omega>0 (A && B) \<omega> RFailure"
 
 \<comment>\<open>exhale A \<longrightarrow> B\<close>
-| ExhImpTrue: 
- "\<lbrakk> ctxt, R, (Some \<omega>0) \<turnstile> \<langle>e; \<omega>\<rangle> [\<Down>]\<^sub>t Val (VBool True); 
+| ExhImpTrue:
+ "\<lbrakk> ctxt, (Some \<omega>0) \<turnstile> \<langle>e; \<omega>\<rangle> [\<Down>]\<^sub>t Val (VBool True);
     red_exhale ctxt R \<omega>0 A \<omega> res \<rbrakk> \<Longrightarrow>
-    red_exhale ctxt R \<omega>0 (Imp e A) \<omega> res" 
-| ExhImpFalse:  
- "\<lbrakk> ctxt, R, (Some \<omega>0) \<turnstile> \<langle>e; \<omega>\<rangle> [\<Down>]\<^sub>t Val (VBool False) \<rbrakk> \<Longrightarrow> 
+    red_exhale ctxt R \<omega>0 (Imp e A) \<omega> res"
+| ExhImpFalse:
+ "\<lbrakk> ctxt, (Some \<omega>0) \<turnstile> \<langle>e; \<omega>\<rangle> [\<Down>]\<^sub>t Val (VBool False) \<rbrakk> \<Longrightarrow>
     red_exhale ctxt R \<omega>0 (Imp e A) \<omega> (RNormal \<omega>)"
 
 \<comment>\<open>exhale e ? A : B\<close>
-| ExhCondTrue: 
- "\<lbrakk> ctxt, R, (Some \<omega>0) \<turnstile> \<langle>e; \<omega>\<rangle> [\<Down>]\<^sub>t Val (VBool True); 
+| ExhCondTrue:
+ "\<lbrakk> ctxt, (Some \<omega>0) \<turnstile> \<langle>e; \<omega>\<rangle> [\<Down>]\<^sub>t Val (VBool True);
     red_exhale ctxt R \<omega>0 A \<omega> res \<rbrakk> \<Longrightarrow>
     red_exhale ctxt R \<omega>0 (CondAssert e A B) \<omega> res"
-| ExhCondFalse: 
- "\<lbrakk> ctxt, R, (Some \<omega>0) \<turnstile> \<langle>e; \<omega>\<rangle> [\<Down>]\<^sub>t Val (VBool False); 
+| ExhCondFalse:
+ "\<lbrakk> ctxt, (Some \<omega>0) \<turnstile> \<langle>e; \<omega>\<rangle> [\<Down>]\<^sub>t Val (VBool False);
     red_exhale ctxt R \<omega>0 B \<omega> res \<rbrakk> \<Longrightarrow>
-    red_exhale ctxt R \<omega>0 (CondAssert e A B) \<omega> res" 
+    red_exhale ctxt R \<omega>0 (CondAssert e A B) \<omega> res"
 
 \<comment>\<open>If a \<^emph>\<open>direct\<close> subexpression is not well-defined, then this results in failure.\<close>
-| ExhSubExpFailure: 
+| ExhSubExpFailure:
   "\<lbrakk> direct_sub_expressions_assertion A \<noteq> [];
-     red_pure_exps_total ctxt R (Some \<omega>0) (direct_sub_expressions_assertion A) \<omega> None  \<rbrakk> \<Longrightarrow> 
+     red_pure_exps_total ctxt R (Some \<omega>0) (direct_sub_expressions_assertion A) \<omega> None  \<rbrakk> \<Longrightarrow>
      red_exhale ctxt R \<omega>0 A \<omega> RFailure"
 
 inductive_cases ExhStar_case: "red_exhale ctxt R \<omega>0 (A && B) m_pm res"
 
-lemma ExhPure_case: 
+lemma ExhPure_case:
   assumes "red_exhale ctxt R \<omega>0 (Atomic (Pure e)) \<omega> res"
-      and "\<And>b. ctxt, R, (Some \<omega>0) \<turnstile> \<langle>e; \<omega>\<rangle> [\<Down>]\<^sub>t Val (VBool b) \<Longrightarrow> res = (exh_if_total b \<omega>) \<Longrightarrow> P"
-      and "ctxt, R, (Some \<omega>0) \<turnstile> \<langle>e; \<omega>\<rangle> [\<Down>]\<^sub>t VFailure \<Longrightarrow> res = RFailure \<Longrightarrow> P"
+      and "\<And>b. ctxt, (Some \<omega>0) \<turnstile> \<langle>e; \<omega>\<rangle> [\<Down>]\<^sub>t Val (VBool b) \<Longrightarrow> res = (exh_if_total b \<omega>) \<Longrightarrow> P"
+      and "ctxt, (Some \<omega>0) \<turnstile> \<langle>e; \<omega>\<rangle> [\<Down>]\<^sub>t VFailure \<Longrightarrow> res = RFailure \<Longrightarrow> P"
     shows "P"
-  using assms 
+  using assms
   by (cases) (auto elim: red_pure_exp_total_elims)
 
 definition havoc_locs_heap :: "'a total_heap \<Rightarrow> heap_loc set \<Rightarrow> 'a total_heap set"
@@ -148,8 +207,8 @@ lemma havoc_locs_heap_empty: "havoc_locs_heap hh {} = {hh}"
 text\<open>\<^term>\<open>havoc_locs_heap hh locs\<close> denotes the set of heaps that differ with \<^term>\<open>hh\<close> only on \<^term>\<open>locs\<close>\<close>
 
 definition havoc_locs_state :: "'a total_context \<Rightarrow> 'a full_total_state \<Rightarrow> heap_loc set \<Rightarrow> 'a full_total_state set"
-  where "havoc_locs_state ctxt \<omega> locs = 
-    { update_hh_total_full \<omega> hh' | (\<omega>' :: 'a full_total_state) (hh' :: 'a total_heap). 
+  where "havoc_locs_state ctxt \<omega> locs =
+    { update_hh_total_full \<omega> hh' | (\<omega>' :: 'a full_total_state) (hh' :: 'a total_heap).
                                    total_heap_well_typed (program_total ctxt) (absval_interp_total ctxt) hh' \<and>
                                    hh' \<in> havoc_locs_heap (get_hh_total_full \<omega>) locs}"
 
@@ -158,7 +217,7 @@ lemma havoc_locs_state_empty:
   shows "\<omega> = \<omega>'"
   using assms
   unfolding havoc_locs_state_def
-  by (simp add: havoc_locs_heap_empty)  
+  by (simp add: havoc_locs_heap_empty)
 
 lemma havoc_locs_state_same_store: "\<omega>' \<in> havoc_locs_state ctxt \<omega> locs \<Longrightarrow> get_store_total \<omega>' = get_store_total \<omega>"
   unfolding havoc_locs_state_def
@@ -172,8 +231,8 @@ lemma havoc_locs_state_same_trace: "\<omega>' \<in> havoc_locs_state ctxt \<omeg
   unfolding havoc_locs_state_def
   by force *)
 
-lemma havoc_locs_state_well_typed_heap: "\<omega>' \<in> havoc_locs_state ctxt \<omega> locs \<Longrightarrow> 
-                                    total_heap_well_typed (program_total ctxt) (absval_interp_total ctxt) (get_hh_total_full \<omega>')"  
+lemma havoc_locs_state_well_typed_heap: "\<omega>' \<in> havoc_locs_state ctxt \<omega> locs \<Longrightarrow>
+                                    total_heap_well_typed (program_total ctxt) (absval_interp_total ctxt) (get_hh_total_full \<omega>')"
 proof -
   assume "\<omega>' \<in> havoc_locs_state ctxt \<omega> locs"
 
@@ -187,25 +246,25 @@ proof -
 qed
 
 inductive fold_rel :: "'a total_context \<Rightarrow> ('a full_total_state \<Rightarrow> bool) \<Rightarrow> predicate_ident \<Rightarrow> ('a val list) \<Rightarrow> preal \<Rightarrow> 'a full_total_state \<Rightarrow> 'a stmt_result_total \<Rightarrow> bool"
-  where 
-    FoldRelNormal: 
+  where
+    FoldRelNormal:
       "\<lbrakk> ViperLang.predicates (program_total ctxt) pred_id = Some pred_decl;
        ViperLang.predicate_decl.body pred_decl = Some pred_body;
        q \<noteq> pnone;
        \<omega>0 = \<lparr> get_store_total = nth_option vs, get_trace_total = Map.empty, get_total_full = get_total_full \<omega> \<rparr>;
        red_exhale ctxt R \<omega>0 (syntactic_mult (Rep_preal q) pred_body) \<omega>0 (RNormal \<omega>1);
-       \<omega>' = \<lparr> get_store_total = get_store_total \<omega>, 
+       \<omega>' = \<lparr> get_store_total = get_store_total \<omega>,
               get_trace_total = get_trace_total \<omega>,
               get_total_full = update_mp_loc_total (get_total_full \<omega>1) (pred_id,vs) (padd (get_mp_total (get_total_full \<omega>1) (pred_id, vs)) q)
-             \<rparr> \<rbrakk> \<Longrightarrow> 
+             \<rparr> \<rbrakk> \<Longrightarrow>
        fold_rel ctxt R pred_id vs q \<omega> (RNormal \<omega>')"
   | FoldRelFailure:
        "\<lbrakk> ViperLang.predicates (program_total ctxt) pred_id = Some pred_decl;
        ViperLang.predicate_decl.body pred_decl = Some pred_body;
        q \<noteq> pnone;
        \<omega>0 = \<lparr> get_store_total = nth_option vs, get_trace_total = Map.empty, get_total_full = get_total_full \<omega> \<rparr>;
-       red_exhale ctxt R \<omega>0 (syntactic_mult (Rep_preal q) pred_body) \<omega>0 RFailure \<rbrakk> \<Longrightarrow> 
-       fold_rel ctxt R pred_id vs q \<omega> RFailure"    
+       red_exhale ctxt R \<omega>0 (syntactic_mult (Rep_preal q) pred_body) \<omega>0 RFailure \<rbrakk> \<Longrightarrow>
+       fold_rel ctxt R pred_id vs q \<omega> RFailure"
 
 inductive_cases FoldRelNormalCase: "fold_rel ctxt R pred_id vs q \<omega> (RNormal \<omega>')"
 inductive_cases FoldRelFailureCase: "fold_rel ctxt R pred_id vs q \<omega> RFailure"
@@ -232,7 +291,7 @@ fun modif :: "stmt \<Rightarrow> var set" where
 | "modif _ = {}"
 
 definition reset_state_after_call :: "var list \<Rightarrow> 'a val list \<Rightarrow> 'a full_total_state \<Rightarrow> 'a full_total_state \<Rightarrow>'a full_total_state" where
-  "reset_state_after_call targets vs \<omega>BeforeCall \<omega> = 
+  "reset_state_after_call targets vs \<omega>BeforeCall \<omega> =
        \<lparr> get_store_total = (map_upds (get_store_total \<omega>BeforeCall) targets vs),
          get_trace_total = get_trace_total \<omega>BeforeCall,
          get_total_full = get_total_full \<omega> \<rparr>"
@@ -240,8 +299,8 @@ definition reset_state_after_call :: "var list \<Rightarrow> 'a val list \<Right
 inductive red_stmt_total :: "'a total_context \<Rightarrow> ('a full_total_state \<Rightarrow> bool) \<Rightarrow> type_context \<Rightarrow> stmt \<Rightarrow> 'a full_total_state  \<Rightarrow> 'a stmt_result_total \<Rightarrow> bool"
   for ctxt :: "'a total_context" and R :: "('a full_total_state \<Rightarrow> bool)" where
 \<comment>\<open>Atomic statements\<close>
-   RedSkip: "red_stmt_total ctxt R \<Lambda> Skip \<omega> (RNormal \<omega>)" 
-| RedInhale: 
+   RedSkip: "red_stmt_total ctxt R \<Lambda> Skip \<omega> (RNormal \<omega>)"
+| RedInhale:
  "\<lbrakk> red_inhale ctxt R A \<omega> res \<rbrakk> \<Longrightarrow>
     red_stmt_total ctxt R \<Lambda> (Inhale A) \<omega> res"
 
@@ -254,7 +313,7 @@ always has at least one failure transition. This is in-sync with the Carbon impl
     \<comment>\<open>We havoc all locations \<^term>\<open>l\<close> for which both of the following conditions hold:
         (1) there is no direct permission to \<^term>\<open>l\<close> after the exhale
         (2) the exhale removed nonzero permission to \<^term>\<open>l\<close>\<close>
-    \<comment>\<open>Once full support for Viper predicates is added, then this exhale semantics needs to also 
+    \<comment>\<open>Once full support for Viper predicates is added, then this exhale semantics needs to also
       take \<^term>\<open>R\<close> into account.\<close> \<rbrakk> \<Longrightarrow>
     red_stmt_total ctxt R \<Lambda> (Exhale A) \<omega> (RNormal \<omega>')"
 | RedExhaleFailure:
@@ -276,57 +335,57 @@ always has at least one failure transition. This is in-sync with the Carbon impl
 \<comment>\<open>only reduce assignment if RHS has the type expected by LHS \<close>
 | RedLocalAssign:
  "\<lbrakk> ctxt, R, (Some \<omega>) \<turnstile> \<langle>e; \<omega>\<rangle> [\<Down>]\<^sub>t (Val v);
-    \<Lambda> x = Some ty; 
-    get_type (absval_interp_total ctxt) v = ty \<rbrakk> \<Longrightarrow> 
+    \<Lambda> x = Some ty;
+    get_type (absval_interp_total ctxt) v = ty \<rbrakk> \<Longrightarrow>
    red_stmt_total ctxt R \<Lambda> (LocalAssign x e) \<omega> (RNormal (update_var_total \<omega> x v))"
-| RedFieldAssign: 
+| RedFieldAssign:
  "\<lbrakk> ctxt, R, (Some \<omega>) \<turnstile> \<langle>e_r; \<omega>\<rangle> [\<Down>]\<^sub>t Val (VRef (Address addr));
     (addr,f) \<in> get_writeable_locs \<omega>;
     ctxt, R, (Some \<omega>)  \<turnstile> \<langle>e; \<omega>\<rangle> [\<Down>]\<^sub>t Val v;
     declared_fields (program_total ctxt) f = Some ty;
-    get_type (absval_interp_total ctxt) v = ty \<rbrakk> \<Longrightarrow> 
+    get_type (absval_interp_total ctxt) v = ty \<rbrakk> \<Longrightarrow>
     red_stmt_total ctxt R \<Lambda> (FieldAssign e_r f e) \<omega> (RNormal (update_hh_loc_total_full \<omega> (addr,f) v))"
 \<comment>\<open>Is null case handled in NestedPermSem?\<close>
-| RedFieldAssignFailure: 
+| RedFieldAssignFailure:
  "\<lbrakk> ctxt, R, (Some \<omega>) \<turnstile> \<langle>e_r; \<omega>\<rangle> [\<Down>]\<^sub>t Val (VRef r);
-    \<comment>\<open>the reduction of the right-hand-side is technically not required for this rule 
+    \<comment>\<open>the reduction of the right-hand-side is technically not required for this rule
        (irrelevant if well-typed), but matches Viper's current reduction order\<close>
-    ctxt, R, (Some \<omega>) \<turnstile> \<langle>e; \<omega>\<rangle> [\<Down>]\<^sub>t Val v; 
-    r = Null \<or> (the_address r,f) \<notin>  get_writeable_locs \<omega> \<rbrakk> \<Longrightarrow> 
+    ctxt, R, (Some \<omega>) \<turnstile> \<langle>e; \<omega>\<rangle> [\<Down>]\<^sub>t Val v;
+    r = Null \<or> (the_address r,f) \<notin>  get_writeable_locs \<omega> \<rbrakk> \<Longrightarrow>
     red_stmt_total ctxt R \<Lambda> (FieldAssign e_r f e) \<omega> RFailure"
 | RedMethodCall:
   " \<lbrakk> red_pure_exps_total ctxt R (Some \<omega>) es \<omega> (Some v_args);
-      program.methods (program_total ctxt) m = Some mdecl;     
+      program.methods (program_total ctxt) m = Some mdecl;
       \<comment>\<open>method call reduces only if argument values and return values have the correct type\<close>
-      vals_well_typed (absval_interp_total ctxt) v_args (method_decl.args mdecl); 
-      list_all2 (\<lambda> y t. y = Some t) (map \<Lambda> ys) (method_decl.rets mdecl); 
+      vals_well_typed (absval_interp_total ctxt) v_args (method_decl.args mdecl);
+      list_all2 (\<lambda> y t. y = Some t) (map \<Lambda> ys) (method_decl.rets mdecl);
       \<comment>\<open>non-deterministically select values for return variables that conform to the declared type\<close>
-      vals_well_typed (absval_interp_total ctxt) v_rets (method_decl.rets mdecl); 
-      red_stmt_total ctxt R \<Lambda> (Exhale (method_decl.pre mdecl)) 
+      vals_well_typed (absval_interp_total ctxt) v_rets (method_decl.rets mdecl);
+      red_stmt_total ctxt R \<Lambda> (Exhale (method_decl.pre mdecl))
                                \<comment>\<open>arguments: 0,1,2,...,n-1\<close>
-                              \<lparr> get_store_total = (shift_and_add_list_alt Map.empty v_args), 
-                                get_trace_total = [old_label \<mapsto> get_total_full \<omega>], 
+                              \<lparr> get_store_total = (shift_and_add_list_alt Map.empty v_args),
+                                get_trace_total = [old_label \<mapsto> get_total_full \<omega>],
                                 get_total_full = get_total_full \<omega> \<rparr>
                               resPre;
       resPre = RFailure \<or> resPre = RMagic \<Longrightarrow> res = resPre;
-      \<And> \<omega>Pre. resPre = RNormal \<omega>Pre \<Longrightarrow> 
+      \<And> \<omega>Pre. resPre = RNormal \<omega>Pre \<Longrightarrow>
       \<comment>\<open>can't use havoc here directly in a natural way to get updated state\<close>
-            (red_stmt_total ctxt R \<Lambda> (Inhale (method_decl.post mdecl))                                     
+            (red_stmt_total ctxt R \<Lambda> (Inhale (method_decl.post mdecl))
                                \<comment>\<open>arguments: 0,1,2,...,n-1 return variables: n,n+1,...\<close>
-                              \<lparr> get_store_total = (shift_and_add_list_alt Map.empty (v_args@v_rets)), 
-                                get_trace_total = [old_label \<mapsto> get_total_full \<omega>], 
+                              \<lparr> get_store_total = (shift_and_add_list_alt Map.empty (v_args@v_rets)),
+                                get_trace_total = [old_label \<mapsto> get_total_full \<omega>],
                                 get_total_full = get_total_full \<omega>Pre \<rparr>
                               resPost \<and>
-            res = map_stmt_result_total (reset_state_after_call ys v_rets \<omega>) resPost) \<rbrakk> \<Longrightarrow>        
+            res = map_stmt_result_total (reset_state_after_call ys v_rets \<omega>) resPost) \<rbrakk> \<Longrightarrow>
       red_stmt_total ctxt R \<Lambda> (MethodCall ys m es) \<omega> res"
  \<comment>\<open>Labels are not overwritten (would not be possible anyway in well-formed programs)\<close>
-| RedLabel:  "\<lbrakk> \<omega>' = (if get_trace_total \<omega> lbl = None then 
-                             update_trace_total \<omega> ((get_trace_total \<omega>)(lbl \<mapsto> get_total_full \<omega>)) 
-                      else \<omega>) \<rbrakk> \<Longrightarrow> 
-              red_stmt_total ctxt R \<Lambda> (Label lbl) \<omega> (RNormal \<omega>')"   
+| RedLabel:  "\<lbrakk> \<omega>' = (if get_trace_total \<omega> lbl = None then
+                             update_trace_total \<omega> ((get_trace_total \<omega>)(lbl \<mapsto> get_total_full \<omega>))
+                      else \<omega>) \<rbrakk> \<Longrightarrow>
+              red_stmt_total ctxt R \<Lambda> (Label lbl) \<omega> (RNormal \<omega>')"
 | RedUnfold:
   "\<lbrakk> red_pure_exps_total ctxt R (Some \<omega>) e_args \<omega> (Some v_args);
-     ctxt, R, (Some \<omega>) \<turnstile> \<langle>e_p; \<omega>\<rangle> [\<Down>]\<^sub>t Val (VPerm v_p);     
+     ctxt, R, (Some \<omega>) \<turnstile> \<langle>e_p; \<omega>\<rangle> [\<Down>]\<^sub>t Val (VPerm v_p);
      W' = {\<omega>'. \<exists>\<phi>'. \<omega>' = \<omega>\<lparr> get_total_full := \<phi>' \<rparr> \<and> unfold_rel ctxt R pred_id v_args (Abs_preal v_p) (get_total_full \<omega>) \<phi>' \<and> R \<omega>'};
      th_result_rel (v_p > 0 \<and> v_p \<le> Rep_preal (get_mp_total_full \<omega> (pred_id, v_args))) True W' res \<rbrakk> \<Longrightarrow>
     red_stmt_total ctxt R \<Lambda> (Unfold pred_id e_args (PureExp e_p)) \<omega> res"
@@ -344,18 +403,18 @@ always has at least one failure transition. This is in-sync with the Carbon impl
 \<comment>\<open>TODO: unfold acc(P(x),0)\<close>
 
 \<comment>\<open>One should be able to prove that if \<omega> is unfolding consistent, then so is \<omega>' after a fold, without
-  explicitly pruning states. This is because folds just replace permissions with a predicate instance 
+  explicitly pruning states. This is because folds just replace permissions with a predicate instance
   (and even if there is a wildcard, we know that there must be at least one transition for the
  newly generated predicate instance, namely the one before the fold)\<close>
 | RedFold:
   "\<lbrakk> red_pure_exps_total ctxt R (Some \<omega>) e_args \<omega> (Some v_args);
-     ctxt, R, (Some \<omega>) \<turnstile> \<langle>e_p; \<omega>\<rangle> [\<Down>]\<^sub>t Val (VPerm v_p);     
+     ctxt, R, (Some \<omega>) \<turnstile> \<langle>e_p; \<omega>\<rangle> [\<Down>]\<^sub>t Val (VPerm v_p);
      fold_rel ctxt R pred_id v_args (Abs_preal v_p) \<omega> res
  \<rbrakk> \<Longrightarrow>
     red_stmt_total ctxt R \<Lambda> (Fold pred_id e_args (PureExp e_p)) \<omega> res"
 
 | RedFoldWildcard:
-  "\<lbrakk> red_pure_exps_total ctxt R (Some \<omega>) e_args \<omega> (Some v_args);     
+  "\<lbrakk> red_pure_exps_total ctxt R (Some \<omega>) e_args \<omega> (Some v_args);
      fold_rel ctxt R pred_id v_args p \<omega> res \<rbrakk> \<Longrightarrow>
     red_stmt_total ctxt R \<Lambda> (Fold pred_id e_args Wildcard) \<omega> res"
 \<comment>\<open>TODO: fold acc(P(x),0)\<close>
@@ -367,30 +426,30 @@ always has at least one failure transition. This is in-sync with the Carbon impl
        res_unshift = map_stmt_result_total (unshift_state_total 1) res \<rbrakk> \<Longrightarrow>
 
       red_stmt_total ctxt R \<Lambda> (Scope \<tau> scopeBody) \<omega> res_unshift"
- | RedIfTrue: 
+ | RedIfTrue:
    "\<lbrakk> ctxt, R, (Some \<omega>) \<turnstile> \<langle>e_b; \<omega>\<rangle> [\<Down>]\<^sub>t Val (VBool True);
-      red_stmt_total ctxt R \<Lambda> s_thn \<omega> res \<rbrakk> \<Longrightarrow> 
+      red_stmt_total ctxt R \<Lambda> s_thn \<omega> res \<rbrakk> \<Longrightarrow>
       red_stmt_total ctxt R \<Lambda> (If e_b s_thn s_els) \<omega> res"
- | RedIfFalse: 
+ | RedIfFalse:
    "\<lbrakk> ctxt, R, (Some \<omega>) \<turnstile> \<langle>e_b; \<omega>\<rangle> [\<Down>]\<^sub>t Val (VBool False);
-      red_stmt_total ctxt R \<Lambda> s_els \<omega> res \<rbrakk> \<Longrightarrow> 
+      red_stmt_total ctxt R \<Lambda> s_els \<omega> res \<rbrakk> \<Longrightarrow>
       red_stmt_total ctxt R \<Lambda> (If e_b s_thn s_els) \<omega> res"
  | RedSeq:
    "\<lbrakk> red_stmt_total ctxt R \<Lambda> s1 \<omega> (RNormal \<omega>');
       red_stmt_total ctxt R \<Lambda> s2 \<omega>' res \<rbrakk> \<Longrightarrow>
       red_stmt_total ctxt R \<Lambda> (Seq s1 s2) \<omega> res"
  | RedSeqFailureOrMagic:
-   "\<lbrakk> red_stmt_total ctxt R \<Lambda> s1 \<omega> res; 
+   "\<lbrakk> red_stmt_total ctxt R \<Lambda> s1 \<omega> res;
       res = RFailure \<or> res = RMagic \<rbrakk> \<Longrightarrow>
       red_stmt_total ctxt R \<Lambda> (Seq s1 s2) \<omega> res"
 (* TODO while loops *)
 \<comment>\<open>Failure subexpression\<close>
-| RedSubExpressionFailure: 
+| RedSubExpressionFailure:
   "\<lbrakk> sub_expressions s \<noteq> [];
-    red_pure_exps_total ctxt R (Some \<omega>) (sub_expressions s) \<omega> None  \<rbrakk> \<Longrightarrow> 
+    red_pure_exps_total ctxt R (Some \<omega>) (sub_expressions s) \<omega> None  \<rbrakk> \<Longrightarrow>
     red_stmt_total ctxt R \<Lambda> s \<omega> RFailure"
 
-inductive_cases RedLocalAssign_case: 
+inductive_cases RedLocalAssign_case:
      "red_stmt_total ctxt R \<Lambda> (LocalAssign x e) \<omega> (RNormal (update_var_total \<omega> x v))"
 
 inductive_cases RedSkip_case: "red_stmt_total ctxt R \<Lambda> Skip \<omega> res"
@@ -428,19 +487,19 @@ subsection \<open>Correctness of Viper methods\<close>
 definition vpr_store_well_typed :: "('a \<Rightarrow> abs_type) \<Rightarrow> type_context \<Rightarrow> 'a store \<Rightarrow> bool"
   where "vpr_store_well_typed A \<Lambda> \<sigma> \<equiv> \<forall>x t. \<Lambda> x = Some t \<longrightarrow> map_option (\<lambda>v. get_type A v) (\<sigma> x) = Some t"
 
-definition vpr_method_correct_total_aux :: 
-          "'a total_context \<Rightarrow> ('a full_total_state \<Rightarrow> bool) \<Rightarrow> method_decl 
-                \<Rightarrow> ('a total_context \<Rightarrow> ('a full_total_state \<Rightarrow> bool) \<Rightarrow> method_decl \<Rightarrow> 'a full_total_state \<Rightarrow> 'a full_total_state \<Rightarrow> bool) 
+definition vpr_method_correct_total_aux ::
+          "'a total_context \<Rightarrow> ('a full_total_state \<Rightarrow> bool) \<Rightarrow> method_decl
+                \<Rightarrow> ('a total_context \<Rightarrow> ('a full_total_state \<Rightarrow> bool) \<Rightarrow> method_decl \<Rightarrow> 'a full_total_state \<Rightarrow> 'a full_total_state \<Rightarrow> bool)
                \<Rightarrow>  bool" where
   "vpr_method_correct_total_aux ctxt R mdecl CorrectWrtPre \<equiv>
-         (\<forall>(\<omega> :: 'a full_total_state) rpre. 
+         (\<forall>(\<omega> :: 'a full_total_state) rpre.
             vpr_store_well_typed (absval_interp_total ctxt) (nth_option (method_decl.args mdecl @ method_decl.rets mdecl)) (get_store_total \<omega>) \<longrightarrow>
             total_heap_well_typed (program_total ctxt) (absval_interp_total ctxt) (get_hh_total_full \<omega>) \<longrightarrow>
             is_empty_total_full \<omega> \<longrightarrow>
             red_inhale ctxt R (method_decl.pre mdecl) \<omega> rpre \<longrightarrow>
             (
               rpre \<noteq> RFailure \<and>
-              (\<forall>\<omega>pre. rpre = RNormal \<omega>pre \<longrightarrow> 
+              (\<forall>\<omega>pre. rpre = RNormal \<omega>pre \<longrightarrow>
                CorrectWrtPre ctxt R mdecl \<omega>pre \<omega>
               )
             )
@@ -466,7 +525,7 @@ definition vpr_postcondition_framed :: "'a total_context \<Rightarrow> ('a full_
                      trace old_label = Some \<phi>pre \<longrightarrow>
                      assertion_framing_state ctxt R postcondition
                              \<lparr> get_store_total = \<sigma>,
-                               get_trace_total = trace, 
+                               get_trace_total = trace,
                                get_total_full = mh \<rparr>
                 )"
 
@@ -483,13 +542,13 @@ lemma vpr_postcondition_framed_assertion_framing_state:
 
 definition vpr_method_body_correct :: "'a total_context \<Rightarrow> ('a full_total_state \<Rightarrow> bool) \<Rightarrow> method_decl \<Rightarrow> 'a full_total_state \<Rightarrow> bool"
   where "vpr_method_body_correct ctxt R mdecl \<omega>pre \<equiv>
-            (\<forall>rbody. red_stmt_total ctxt R 
+            (\<forall>rbody. red_stmt_total ctxt R
                                 (nth_option (method_decl.args mdecl @ method_decl.rets mdecl))
                                 (Seq (the (method_decl.body mdecl)) (Exhale (method_decl.post mdecl)))
-                                (update_trace_total \<omega>pre (Map.empty(old_label \<mapsto> get_total_full \<omega>pre))) 
+                                (update_trace_total \<omega>pre (Map.empty(old_label \<mapsto> get_total_full \<omega>pre)))
                                 rbody \<longrightarrow> rbody \<noteq> RFailure)
-                        \<comment>\<open>  (rbody \<noteq> RFailure \<and> 
-                            (\<forall>\<omega>body. rbody = RNormal \<omega>body \<longrightarrow> 
+                        \<comment>\<open>  (rbody \<noteq> RFailure \<and>
+                            (\<forall>\<omega>body. rbody = RNormal \<omega>body \<longrightarrow>
                                 (\<forall> rpost. red_exhale ctxt R \<omega>body (method_decl.post mdecl) \<omega>body rpost \<longrightarrow> rpost \<noteq> RFailure)
                             )
                           )\<close>
@@ -498,8 +557,8 @@ definition vpr_method_body_correct :: "'a total_context \<Rightarrow> ('a full_t
 
 definition vpr_method_correct_total :: "'a total_context \<Rightarrow> ('a full_total_state \<Rightarrow> bool) \<Rightarrow> method_decl \<Rightarrow> bool" where
   "vpr_method_correct_total ctxt R mdecl \<equiv>
-         vpr_method_correct_total_aux ctxt R mdecl 
-          (\<lambda>ctxt R mdecl \<omega>pre \<omega>. 
+         vpr_method_correct_total_aux ctxt R mdecl
+          (\<lambda>ctxt R mdecl \<omega>pre \<omega>.
                 vpr_postcondition_framed ctxt R (method_decl.post mdecl) (get_total_full \<omega>pre) (get_store_total \<omega>) \<and>
                 (\<forall>mbody. method_decl.body mdecl = Some mbody \<longrightarrow> vpr_method_body_correct ctxt R mdecl \<omega>pre)
           )
@@ -507,14 +566,14 @@ definition vpr_method_correct_total :: "'a total_context \<Rightarrow> ('a full_
 
 definition vpr_method_correct_total_expanded :: "'a total_context \<Rightarrow> ('a full_total_state \<Rightarrow> bool) \<Rightarrow> method_decl \<Rightarrow> bool" where
   "vpr_method_correct_total_expanded ctxt R mdecl \<equiv>
-         (\<forall>(\<omega> :: 'a full_total_state) rpre. 
+         (\<forall>(\<omega> :: 'a full_total_state) rpre.
             vpr_store_well_typed (absval_interp_total ctxt) (nth_option (method_decl.args mdecl @ method_decl.rets mdecl)) (get_store_total \<omega>) \<longrightarrow>
             total_heap_well_typed (program_total ctxt) (absval_interp_total ctxt) (get_hh_total_full \<omega>) \<longrightarrow>
             is_empty_total_full \<omega> \<longrightarrow>
             red_inhale ctxt R (method_decl.pre mdecl) \<omega> rpre \<longrightarrow>
             (
               rpre \<noteq> RFailure \<and>
-              (\<forall>\<omega>pre. rpre = RNormal \<omega>pre \<longrightarrow> 
+              (\<forall>\<omega>pre. rpre = RNormal \<omega>pre \<longrightarrow>
                 \<comment>\<open>\<^term>\<open>get_store_total \<omega>\<close> should be equal to \<^term>\<open>get_store_total \<omega>pre\<close> since inhale does not change the store.\<close>
                 vpr_postcondition_framed ctxt R (method_decl.post mdecl) (get_total_full \<omega>pre) (get_store_total \<omega>) \<and>
                 (\<forall>mbody. method_decl.body mdecl = Some mbody \<longrightarrow> vpr_method_body_correct ctxt R mdecl \<omega>pre)
@@ -537,8 +596,8 @@ lemma vpr_method_correct_total_2_new_equiv:
 
 definition vpr_method_spec_correct_total :: "'a total_context \<Rightarrow> ('a full_total_state \<Rightarrow> bool) \<Rightarrow> method_decl \<Rightarrow> bool" where
   "vpr_method_spec_correct_total ctxt R mdecl \<equiv>
-         vpr_method_correct_total_aux ctxt R mdecl 
-          (\<lambda>ctxt R mdecl \<omega>pre \<omega>. 
+         vpr_method_correct_total_aux ctxt R mdecl
+          (\<lambda>ctxt R mdecl \<omega>pre \<omega>.
                 vpr_postcondition_framed ctxt R (method_decl.post mdecl) (get_total_full \<omega>pre) (get_store_total \<omega>)
           )
        "
@@ -552,7 +611,7 @@ lemma vpr_method_spec_correct_total_from_all:
     shows "vpr_method_spec_correct_total ctxt R mdecl"
   using assms
   unfolding vpr_all_method_spec_correct_total_def
-  by blast    
+  by blast
 
 subsection \<open>Alternative introduction rules\<close>
 
@@ -598,13 +657,13 @@ text \<open>Many of the theorems are parametrized by the state consistency. Many
 certain properties on the state consistency. The following well-formedness definition captures
 these properties.\<close>
 
-(* definition wf_total_consistency 
-  where "wf_total_consistency ctxt R Rt \<equiv> 
+(* definition wf_total_consistency
+  where "wf_total_consistency ctxt R Rt \<equiv>
                mono_prop_downward R \<and>
                (\<forall>\<omega>. is_empty_total_full \<omega> \<longrightarrow> R \<omega>) \<and>
                (\<forall>\<omega> \<omega>' \<Lambda> stmt. R \<omega> \<longrightarrow> red_stmt_total ctxt R \<Lambda> stmt \<omega> (RNormal \<omega>') \<longrightarrow> R \<omega>') \<and>
                \<comment>\<open>The following statement ensures that states in the body of a scope preserve consistency.\<close>
-               (\<forall>\<omega> v. R \<omega> \<longrightarrow> R (shift_and_add_state_total \<omega> v)) \<and> 
+               (\<forall>\<omega> v. R \<omega> \<longrightarrow> R (shift_and_add_state_total \<omega> v)) \<and>
                (\<forall>\<omega>. R \<omega> \<longleftrightarrow> (Rt (get_total_full \<omega>) \<and> (\<forall>lbl \<phi>. get_trace_total \<omega> lbl = Some \<phi> \<longrightarrow> Rt \<phi>)) )"
 
 lemma total_consistencyI:
@@ -621,7 +680,7 @@ lemma wf_total_consistency_trivial: "wf_total_consistency ctxt (\<lambda>_.True)
   by blast
 
 lemma total_consistency_red_stmt_preserve:
-  assumes "wf_total_consistency ctxt R Rt" 
+  assumes "wf_total_consistency ctxt R Rt"
       and "R \<omega>"
       and "red_stmt_total ctxt R \<Lambda> stmt \<omega> (RNormal \<omega>')"
     shows "R \<omega>'"
@@ -630,9 +689,9 @@ lemma total_consistency_red_stmt_preserve:
   by blast
 
 lemma total_consistency_store_update:
-  assumes "wf_total_consistency ctxt R Rt" 
-      and "R \<omega>" 
-      and "get_total_full \<omega>' = get_total_full \<omega>" 
+  assumes "wf_total_consistency ctxt R Rt"
+      and "R \<omega>"
+      and "get_total_full \<omega>' = get_total_full \<omega>"
       and "get_trace_total \<omega>' = get_trace_total \<omega>"
     shows "R \<omega>'"
   using assms
@@ -640,29 +699,29 @@ lemma total_consistency_store_update:
   by metis
 
 lemma total_consistency_store_update_2:
-  assumes "wf_total_consistency ctxt R Rt" 
-      and "R \<omega>" 
+  assumes "wf_total_consistency ctxt R Rt"
+      and "R \<omega>"
     shows "R (\<omega> \<lparr> get_store_total := \<sigma> \<rparr>)"
   using assms total_consistency_store_update
   by fastforce
 
 lemma total_consistency_trace_update:
-  assumes "wf_total_consistency ctxt R Rt" 
-      and "R \<omega>" 
+  assumes "wf_total_consistency ctxt R Rt"
+      and "R \<omega>"
       and "get_store_total \<omega>' = get_store_total \<omega>"
-      and "get_total_full \<omega>' = get_total_full \<omega>" 
+      and "get_total_full \<omega>' = get_total_full \<omega>"
       and "\<And> lbl \<phi>. get_trace_total \<omega>' lbl = Some \<phi> \<Longrightarrow> Rt \<phi>"
     shows "R \<omega>'"
-  using assms 
+  using assms
   unfolding wf_total_consistency_def
   by simp
 
 lemma total_consistency_trace_update_2:
-  assumes "wf_total_consistency ctxt R Rt" 
-      and "R \<omega>" 
+  assumes "wf_total_consistency ctxt R Rt"
+      and "R \<omega>"
       and "\<And> lbl \<phi>. t lbl = Some \<phi> \<Longrightarrow> Rt \<phi>"
     shows "R (\<omega> \<lparr> get_trace_total := t \<rparr>)"
-  using assms 
+  using assms
   unfolding wf_total_consistency_def
   by simp
 
@@ -676,7 +735,7 @@ lemma wf_total_consistency_trace_mono_downwardD:
 subsection \<open>Experimental definitions\<close>
 
 definition assertion_sat :: "'a total_context \<Rightarrow> ('a full_total_state \<Rightarrow> bool) \<Rightarrow> type_context \<Rightarrow> assertion \<Rightarrow> 'a full_total_state \<Rightarrow> bool"
-  where "assertion_sat \<Lambda> R ctxt A \<omega> = 
+  where "assertion_sat \<Lambda> R ctxt A \<omega> =
             (\<forall> res. red_stmt_total \<Lambda> R ctxt (Assert A) \<omega> res \<longrightarrow> res \<noteq> RFailure)"
 
 text \<open>Note that \<^const>\<open>assertion_sat\<close> is ``demonic'', i.e., every reduction of asserting \<^term>\<open>A\<close> must
@@ -684,18 +743,18 @@ be a non-failing state, which is in-sync with the semantics of assert statements
 want to change both to be ``locally angelic''. \<close>
 
 definition heap_dep_interp_wf :: "'a total_context \<Rightarrow> ('a full_total_state \<Rightarrow> bool) \<Rightarrow> type_context \<Rightarrow> bool"
-  where 
-    "heap_dep_interp_wf ctxt StateCons \<Lambda> \<equiv> \<forall>fid fdecl. ViperLang.funs (program_total ctxt) fid = Some fdecl \<longrightarrow> 
+  where
+    "heap_dep_interp_wf ctxt StateCons \<Lambda> \<equiv> \<forall>fid fdecl. ViperLang.funs (program_total ctxt) fid = Some fdecl \<longrightarrow>
        (\<exists>fsem. fun_interp_total ctxt fid = Some fsem \<and>
-            (\<forall>vs \<omega>.   
+            (\<forall>vs \<omega>.
                ( ( \<not>vals_well_typed (absval_interp_total ctxt) vs (args fdecl) ) \<longrightarrow> fsem vs \<omega> = None) \<and>
 
-               ( 
+               (
                  ( vals_well_typed (absval_interp_total ctxt) vs (args fdecl) \<and> assertion_self_framing_store ctxt StateCons (pre fdecl) (nth_option vs) ) \<longrightarrow>
 
                      ( (\<not>assertion_sat ctxt StateCons \<Lambda> (pre fdecl) (update_store_total \<omega> (nth_option vs))) \<longrightarrow>
                            fsem vs \<omega> = Some VFailure ) \<and>
-  
+
                      (assertion_sat ctxt StateCons \<Lambda> (pre fdecl) (update_store_total \<omega> (nth_option vs)) \<longrightarrow>
                          (\<exists>v. fsem vs \<omega> = Some (Val v) \<and> get_type (absval_interp_total ctxt) v = ret fdecl \<and>
                               if_Some (\<lambda>e. ctxt, StateCons, (Some \<omega>) \<turnstile> \<langle>e;\<omega>\<rangle> [\<Down>]\<^sub>t (Val v)) (body fdecl) ) )
@@ -705,9 +764,9 @@ definition heap_dep_interp_wf :: "'a total_context \<Rightarrow> ('a full_total_
 
 definition heap_dep_fun_obligations :: "'a total_context \<Rightarrow> ('a full_total_state \<Rightarrow> bool) \<Rightarrow> type_context \<Rightarrow> bool"
   where
-    "heap_dep_fun_obligations ctxt StateCons \<Lambda> \<equiv> 
-       \<forall> fid fdecl vs e p. 
-          ( ViperLang.funs (program_total ctxt) fid = Some fdecl \<and>            
+    "heap_dep_fun_obligations ctxt StateCons \<Lambda> \<equiv>
+       \<forall> fid fdecl vs e p.
+          ( ViperLang.funs (program_total ctxt) fid = Some fdecl \<and>
             body fdecl = Some e \<and>
             vals_well_typed (absval_interp_total ctxt) vs (args fdecl) \<and>
             post fdecl = Some p)  \<longrightarrow>
@@ -715,7 +774,7 @@ definition heap_dep_fun_obligations :: "'a total_context \<Rightarrow> ('a full_
               assertion_self_framing_store ctxt StateCons (pre fdecl) (nth_option vs) \<and>
                 (\<forall> \<omega> extVal.
                   assertion_sat ctxt StateCons \<Lambda> (pre fdecl) (update_store_total \<omega> (nth_option vs)) \<longrightarrow>
-    
+
                     ctxt, StateCons, (Some (update_store_total \<omega> (nth_option vs))) \<turnstile> \<langle>e; (update_store_total \<omega> (nth_option vs))\<rangle> [\<Down>]\<^sub>t extVal \<and>
                       ((\<exists> v. extVal = Val v \<and>
                          assertion_sat ctxt StateCons \<Lambda> p (update_store_total \<omega> (nth_option (vs@[v])))))
@@ -734,7 +793,7 @@ definition predicate_obligations :: "'a total_context \<Rightarrow> ('a full_tot
 (* TODO loops
 
 definition havoc_vars_state :: "'a full_total_state \<Rightarrow> var set \<Rightarrow> 'a full_total_state set"
-  where "havoc_vars_state \<omega> havoced_vars = { update_store_total \<omega> \<sigma>' | \<sigma>'. 
+  where "havoc_vars_state \<omega> havoced_vars = { update_store_total \<omega> \<sigma>' | \<sigma>'.
                                       dom \<sigma>' = dom (get_store_total \<omega>) \<and>
                                       (\<forall> x \<in> dom (get_store_total \<omega>) - havoced_vars. get_store_total \<omega> x = \<sigma>' x) }"
  | RedWhile:
@@ -743,8 +802,8 @@ definition havoc_vars_state :: "'a full_total_state \<Rightarrow> var set \<Righ
           (ctxt, R, (Some \<omega>AfterHavoc) \<turnstile> \<langle>cond; \<omega>AfterHavoc\<rangle> [\<Down>]\<^sub>t Val (VBool True) \<Longrightarrow>
           red_inhale ctxt R invariant \<omega>AfterHavoc (RNormal \<omega>AfterInh) \<Longrightarrow>
           red_stmt_total ctxt R \<Lambda> loop_body \<omega>AfterInh (RNormal \<omega>AfterBody) \<Longrightarrow>
-          red_stmt_total ctxt R \<Lambda> (Assert invariant) \<omega>AfterBody res \<Longrightarrow> 
-          res \<noteq> RFailure))      
+          red_stmt_total ctxt R \<Lambda> (Assert invariant) \<omega>AfterBody res \<Longrightarrow>
+          res \<noteq> RFailure))
        \<rbrakk> \<Longrightarrow>
       red_stmt_total ctxt R \<Lambda> (While cond invariant loop_body) \<omega> \<omega>'"
 
@@ -758,10 +817,10 @@ definition havoc_vars_state :: "'a full_total_state \<Rightarrow> var set \<Righ
 \<comment>\<open>TODO: intermediate failures\<close>
   | RedWhileFailure:
    "\<lbrakk> red_stmt_total ctxt R \<Lambda> (Exhale invariant) \<omega> (RNormal \<omega>AfterExh); \<comment>\<open>failure option 1\<close>
-      \<omega>AfterHavoc \<in> havoc_vars_state \<omega>AfterExh (modif loop_body); 
+      \<omega>AfterHavoc \<in> havoc_vars_state \<omega>AfterExh (modif loop_body);
       red_inhale ctxt R invariant                                       \<comment>\<open>failure option 2\<close>
-            (empty_full_total_state 
-                        (get_store_total \<omega>AfterHavoc) 
+            (empty_full_total_state
+                        (get_store_total \<omega>AfterHavoc)
                         (get_trace_total \<omega>AfterHavoc)
                         (get_h_total_full \<omega>AfterHavoc))
             (RNormal \<omega>AfterInh);
