viper-total-heaps/TotalSemanticsCore.thy
@@ -15,6 +15,8 @@ record 'a total_context =
   fun_interp_total :: "'a interp"
   absval_interp_total :: "'a \<Rightarrow> abs_type"
 
+datatype 'a result_total = RMagic | RFailure | RNormal "'a full_total_state"
+
 
 subsection \<open>Shift Operations\<close>
 
@@ -195,13 +197,13 @@ inductive red_pure_exp_total :: "'a total_context \<Rightarrow> 'a full_total_st
 \<comment>\<open>
 \<comment>\<open>Function application\<close>
 | RedFunApp: (* Should function application be expressed operationally? *)
-   "\<lbrakk> (fun_interp_total ctxt) fname = Some f;
-      red_pure_exps_total ctxt R \<omega>_def es \<omega> (Some vs);
-      \<comment>\<open>TODO: The precondition of a function needs to be checked w.r.t. the well-definedness state.
-               One could define two interpretations of the function, one that checks the precondition
-               and one that does not.\<close>
-      f vs \<omega> = Some res \<rbrakk> \<Longrightarrow>
-      ctxt, \<omega>_def \<turnstile> \<langle>FunApp fname es; \<omega>\<rangle> [\<Down>] res"
+  "\<lbrakk> (fun_interp_total ctxt) fname = Some f;
+     red_pure_exps_total ctxt \<omega>_def es \<omega> (Some vs);
+     \<comment>\<open>TODO: The precondition of a function needs to be checked w.r.t. the well-definedness state.
+              One could define two interpretations of the function, one that checks the precondition
+              and one that does not.\<close>
+     f vs \<omega> = Some res \<rbrakk> \<Longrightarrow>
+   ctxt, \<omega>_def \<turnstile> \<langle>FunApp fname es; \<omega>\<rangle> [\<Down>] res"
 \<close>
 
 \<comment>\<open>Permission introspection\<close>
@@ -246,6 +248,77 @@ inductive red_pure_exp_total :: "'a total_context \<Rightarrow> 'a full_total_st
    red_pure_exps_total ctxt \<omega>_def (e#es) \<omega> None"
 | RedExpListNil:
   "red_pure_exps_total ctxt \<omega>_def Nil \<omega> (Some Nil)"
+
+
+subsection \<open>Inhale\<close>
+
+definition inhale_perm_single :: "'a full_total_state \<Rightarrow> heap_loc \<Rightarrow> preal option \<Rightarrow> 'a full_total_state set"
+  where "inhale_perm_single \<omega> lh p_opt =
+    { \<omega>'| \<omega>' q.
+            option_fold ((=) q) (q \<noteq> pnone) p_opt \<and>
+            get_mh_total_full \<omega> lh + q \<le> 1 \<and>  \<comment> \<open>There can be at most 1 field permission\<close>
+               \<comment> \<open>Do we really need the check here? Or it is covered in consistency?\<close>
+            \<omega>' = update_mh_loc_total_full \<omega> lh ((get_mh_total_full \<omega> lh) + q)
+    }"
+
+inductive red_inhale :: "'a total_context \<Rightarrow> assertion \<Rightarrow> 'a full_total_state \<Rightarrow> 'a result_total \<Rightarrow> bool" where
+\<comment>\<open>Atomic inhale\<close>
+InhAcc:
+  "\<lbrakk> ctxt, Some \<omega> \<turnstile> \<langle>e_r; \<omega>\<rangle> [\<Down>]\<^sub>t Val (VRef r);
+     ctxt, Some \<omega> \<turnstile> \<langle>e_p; \<omega>\<rangle> [\<Down>]\<^sub>t Val (VPerm p);
+     W' = (if r = Null then {\<omega>} else inhale_perm_single \<omega> (the_address r,f) (Some (Abs_preal p)));
+     th_result_rel (p \<ge> 0) (W' \<noteq> {} \<and> (p > 0 \<longrightarrow> r \<noteq> Null)) W' res \<rbrakk> \<Longrightarrow>
+   red_inhale ctxt (Atomic (Acc e_r f (PureExp e_p))) \<omega> res"
+| InhAccPred:
+  "\<lbrakk> red_pure_exps_total ctxt (Some \<omega>) e_args \<omega> (Some v_args);
+     ctxt, Some \<omega> \<turnstile> \<langle>e_p; \<omega>\<rangle> [\<Down>]\<^sub>t Val (VPerm p);
+     W' = inhale_perm_single_pred \<omega> (pred_id, v_args) (Some (Abs_preal p));
+     th_result_rel (p \<ge> 0) (W' \<noteq> {}) W' res \<rbrakk> \<Longrightarrow>
+   red_inhale ctxt (Atomic (AccPredicate pred_id e_args (PureExp e_p))) \<omega> res"
+| InhAccWildcard:
+  "\<lbrakk> ctxt, Some \<omega> \<turnstile> \<langle>e_r; \<omega>\<rangle> [\<Down>]\<^sub>t Val (VRef r);
+     W' = inhale_perm_single \<omega> (the_address r,f) None;
+     th_result_rel True (W' \<noteq> {} \<and> r \<noteq> Null) W' res \<rbrakk> \<Longrightarrow>
+   red_inhale ctxt (Atomic (Acc e_r f Wildcard)) \<omega> res"
+| InhAccPredWildcard:
+  "\<lbrakk> red_pure_exps_total ctxt (Some \<omega>) e_args \<omega> (Some v_args);
+     W' = inhale_perm_single_pred \<omega> (pred_id, v_args) None;
+     th_result_rel True (W' \<noteq> {}) W' res \<rbrakk> \<Longrightarrow>
+   red_inhale ctxt (Atomic (AccPredicate pred_id e_args Wildcard)) \<omega> res"
+| InhPure:
+  "\<lbrakk> ctxt, Some \<omega> \<turnstile> \<langle>e; \<omega>\<rangle> [\<Down>]\<^sub>t Val (VBool b) \<rbrakk> \<Longrightarrow>
+   red_inhale ctxt (Atomic (Pure e)) \<omega> (if b then RNormal \<omega> else RMagic)"
+
+\<comment>\<open>Connectives inhale\<close>
+| InhStarNormal:
+  "\<lbrakk> red_inhale ctxt A \<omega> (RNormal \<omega>'');
+     red_inhale ctxt B \<omega>'' res\<rbrakk> \<Longrightarrow>
+   red_inhale ctxt (A && B) \<omega> res"
+| InhStarFailureMagic:
+  "\<lbrakk> red_inhale ctxt A \<omega> resA;
+     resA = RFailure \<or> resA = RMagic \<rbrakk> \<Longrightarrow>
+   red_inhale ctxt (A && B) \<omega> resA"
+| InhImpTrue:
+  "\<lbrakk> ctxt, Some \<omega> \<turnstile> \<langle>e; \<omega>\<rangle> [\<Down>]\<^sub>t (Val (VBool True));
+     red_inhale ctxt A \<omega> res \<rbrakk> \<Longrightarrow>
+   red_inhale ctxt (Imp e A) \<omega> res"
+| InhImpFalse:
+  "\<lbrakk> ctxt, Some \<omega> \<turnstile> \<langle>e; \<omega>\<rangle> [\<Down>]\<^sub>t Val (VBool False) \<rbrakk> \<Longrightarrow>
+   red_inhale ctxt (Imp e A) \<omega> (RNormal \<omega>)"
+| InhCondAssertTrue:
+  "\<lbrakk> ctxt, Some \<omega> \<turnstile> \<langle>e; \<omega>\<rangle> [\<Down>]\<^sub>t (Val (VBool True));
+    red_inhale ctxt A \<omega> res \<rbrakk> \<Longrightarrow>
+   red_inhale ctxt (CondAssert e A B) \<omega> res"
+| InhCondAssertFalse:
+  "\<lbrakk> ctxt, Some \<omega> \<turnstile> \<langle>e; \<omega>\<rangle> [\<Down>]\<^sub>t Val (VBool False);
+    red_inhale ctxt B \<omega> res \<rbrakk> \<Longrightarrow>
+   red_inhale ctxt (CondAssert e A B) \<omega> res"
+
+\<comment>\<open>If a \<^emph>\<open>direct\<close> subexpression is not well-defined, then this result in failure.\<close>
+| InhSubExpFailure:
+  "\<lbrakk> (direct_sub_expressions_assertion A) \<noteq> [];
+     red_pure_exps_total ctxt (Some \<omega>) (direct_sub_expressions_assertion A) \<omega> None \<rbrakk> \<Longrightarrow>
+   red_inhale ctxt A \<omega> RFailure"
 
 
 subsection \<open>Unfold\<close>
